src/test/interop/memcpy/Memcpy.fst
@@ -1,0 +1,20 @@
+module Memcpy
+
+open FStar.Pointer.Base
+
+let bytes = buffer UInt8.t
+
+assume val memcpy_8: src:bytes -> srci:UInt32.t -> dest:bytes -> desti:UInt32.t -> len:UInt32.t ->
+  STL unit 
+  (requires (fun h -> live #UInt8.t h src /\ live #UInt8.t h dest /\ disjoint src dest 
+    /\ length #UInt8.t src >= UInt32.v srci + UInt32.v len /\ length #UInt8.t dest >= UInt32.v desti + UInt32.v len))
+  (ensures  (fun h0 _ h1 -> live #UInt8.t h0 src /\ live #UInt8.t h0 dest /\ live #UInt8.t h1 dest /\ modifies_1 dest h0 h1
+    /\ length #UInt8.t src >= UInt32.v srci + UInt32.v len 
+    /\ length #UInt8.t dest >= UInt32.v desti + UInt32.v len
+    /\ (let d1 = to_seq #UInt8.t h1 dest in let d0 = to_seq #UInt8.t h0 dest in let s0 = to_seq #UInt8.t h0 src in
+        Seq.slice d1 0 (UInt32.v desti) == Seq.slice d0 0 (UInt32.v desti)
+	/\ Seq.slice d1 (UInt32.v desti) (UInt32.v desti + UInt32.v len) ==
+	    Seq.slice s0 (UInt32.v srci) (UInt32.v srci + UInt32.v len)
+	/\ Seq.slice d1 (UInt32.v desti + UInt32.v len) (length #UInt8.t dest) ==
+	    Seq.slice d0 (UInt32.v desti + UInt32.v len) (length #UInt8.t dest)) ))
+  
